\section{Spectral relations}

From the equivalent definition given by Rodrigues' formula
\[
  P_{n}^{(a,b)}(z) = \frac{(-1)^n}{2^nn!} (1-z)^{-a}(1+z)^{-b}
  \frac{d^n}{dz^n} (1-z)^{a+n}(1+z)^{b+n},
\]
the Fourier transform of $Q_n^{(a,b)}(z) = (1-z)^a(1+z)^bP_n^{(a,b)}(z)$
restricted on the interval $[-1,1]$ is 
\begin{align*}
  \int_{-1}^1 e^{-i\xi x} Q_n^{(a,b)}(x)dx
  %  = \frac{(-1)^n}{2^nn!} \int_{-1}^1 e^{-i\xi x} 
  %\frac{d^n}{dx^n} (1-x)^{a+n}(1+x)^{b+n} dx
  = \frac{(-i\xi)^n}{2^nn!}\int_{-1}^1 e^{-i\xi x} (1-x)^{a+n}(1+x)^{b+n}dx,
\end{align*}
using integration by parts repeatedly. Using the change of variable $x = 2\eta-1$, the last 
integral becomes 
\begin{align*}
  &\quad \frac{(-i\xi)^n}{n!} 2^{a+b+n+1}e^{i\xi}
  \int_0^1 e^{-2i\xi\eta}(1-\eta)^{a+n}\eta^{b+n} d\eta\cr
  &= \frac{(-i\xi)^n}{n!} 2^{a+b+n+1}e^{i\xi}\sum_{k=0}^\infty \frac{(-2i\xi)^k}{k!}
  \int_0^1 (1-\eta)^{a+b}\eta^{b+n+k}d\eta\cr
  &= 
  \frac{(-i\xi)^n}{n!} 2^{a+b+n+1}e^{i\xi}\sum_{k=0}^\infty \frac{(-2i\xi)^k}{k!}
  \frac{\Gamma(a+n+1)\Gamma(b+n+k+1)}{\Gamma(a+b+2n+k+2)} \cr
%  \int_0^1 (1-\eta)^{a+n}\eta^{b+n+k}d\eta\cr
  &= \frac{(-i\xi)^n}{n!} 2^{a+b+n+1}e^{i\xi}B(a+n+1,b+n+1)
  { }_1F_1(b+n+1;a+b+2n+2;-2i\xi).
\end{align*}
where $\Gamma(z)$ is the Euler Gamma function, $B(a,b)=\int_0^1 \eta^{a-1}(1-\eta)^{b-1}d\eta
=\frac{\Gamma(a)\Gamma(b)}{\Gamma(a+b)}$ is the Beta function
and ${ }_1F_1(a;b;z)$ is the confluence hypergeometric function.

Because of $\mathcal{A}Q_n^{(a,b)}$ is a real function, its representation as 
an inverse Fourier transform can be  written as 
\begin{multline}
  \mathcal{A}Q_n^{(a,b)} = \frac{1}{\pi} \Re \int_0^\infty 
  e^{ix\xi} \psi(\xi) \widehat{Q_n^{(a,b)}}(\xi)d\xi 
  = \frac{2^{a+b+n+1}}{\pi n!}B(a+n+1,b+n+1)\cr
  \Re\left[ e^{-i\pi\gamma} (-i)^n
  \int_0^\infty \xi^{n+\alpha} e^{i(x+1)\xi}
{ }_1F_1(b+n+1;a+b+2n+2;-2i\xi)d\xi\right].
\label{eq:infaq}
\end{multline}
From the asymptotic expansion 
\begin{align*}
    { }_1F_1(a;b;-2iz) 
    %&= \frac{\Gamma(b)}{\Gamma(a)\Gamma(b-a)}
    %  \int_0^1 e^{-2iuz} u^{a-1}(1-u)^{b-a-1}du \cr
    =\frac{\Gamma(b)}{\Gamma(b-a)}
    \sum_{k=0}^\infty \frac{(a+1-b)_k(a)_k}{k!}(2iz)^{-a-k}
    +\frac{\Gamma(b)}{\Gamma(a)}
    e^{-2i\xi} \sum_{k=0}^\infty \frac{(1-a)_k(b-a)_k}{k!}(-2iz)^{a-b-k},
  \end{align*}
  the last integral in Eq.~\eqref{eq:infaq} is convergent for 
  $\alpha \in (-n-1, \min(a+1,b+1))$.
\begin{lem}
\end{lem}

